wip

src/Thread.v
@@ -18,9 +18,9 @@ From ExtLib Require Import
 From ITree Require Import
      ITree
      ITreeFacts
-     Events.MapDefault
-     Events.StateFacts
-     Events.Nondeterminism.
+     Events.Exception
+     Events.Nondeterminism
+     Events.State.
 
 (* The [sum1] types with automatic application of commutativity and
    associativity are prone to infinite instance resolution loops.
@@ -60,49 +60,96 @@ Module Denote (Arc : ArcSig).
                    write_kind : Arc.InsSem.mem_read_kind }.
 
 
+  Variant storageE : Type -> Type :=
+
   Variant threadE : Type -> Type :=
   | ThEInsFetch : Arc.InsSem.pc_t -> threadE Arc.InsSem.machine_code
   | ThEInsDecode : Arc.InsSem.machine_code -> threadE Arc.InsSem.ast
   | ThEInsNextLocs : Arc.InsSem.pc_t -> Arc.InsSem.ast ->
-                     threadE (list (instruction_id_t * Arc.InsSem.pc_t)).
-  (* | ThEInsSem : forall A, Arc.InsSem.E A -> threadE A. *)
+                     threadE (list (instruction_id_t * Arc.InsSem.pc_t))
+  | ThEInsFinish : threadE unit
+  (* Load instruction *)
+  | ThEInsInitReads : Arc.mem_slc -> threadE (list mem_read_id_t)
+  | ThEInsWriteForward : mem_read_id_t -> threadE bool
+  | ThEInsReadFromSto : mem_read_id_t -> threadE bool
+  | ThEGetValueOfReads : threadE Arc.mem_slc_val.
+  (* | ThEInsSem : forall A, Arc.InsSem.E A -> threadE (option A). *)
   (* Arguments ThEInsSem {A}. *)
 
-  Context {E: Type -> Type}.
-  Context `{wrapE threadE instruction_id_t -< E}.
-  Context `{wrapE Arc.InsSem.E instruction_id_t -< E}.
+  Definition handle_regE {E} `{threadE -< E} `{nondetFinE -< E}
+    : Arc.InsSem.regE ~> itree E :=
+    fun _ e =>
+      match e with
+      | Arc.InsSem.RegERead rslc => ITree.spin (* FIXME: *)
+      | Arc.InsSem.RegEWrite rslc rval => ITree.spin (* FIXME: *)
+      end.
 
-  Definition SE := nondet_schedulerE (instruction_id_t * Arc.InsSem.pc_t) +' E.
+  Definition handle_mem_read {E} `{threadE -< E} `{nondetFinE -< E}
+             (slc : Arc.mem_slc) : itree E Arc.mem_slc_val :=
+    rids <- trigger (ThEInsInitReads slc)
+    ;; ITree.iter (fun rids (* rids that aren't fully satisfied yet *) =>
+                     match rids with
+                     | [] => (* All the reads are satisfied *)
+                       v <- trigger ThEGetValueOfReads
+                       ;; ret (inr v)
+                     | _ =>
+                       rid <- choose rids
+                       ;; read_event <- choose [ThEInsWriteForward rid;
+                                              ThEInsReadFromSto rid]
+                       ;; is_sat <- trigger read_event
+                       ;; ret (inl (if (is_sat : bool) then List.remove Nat.eq_dec rid rids else rids))
+                     end) rids.
 
-  (* Definition handle_regE {E} *)
-  (*   : wrapE Arc.InsSem.regE instruction_id_t ~> itree E := *)
-  (*   fun _ e => *)
-  (*     let '(Wrap e iid) := e in *)
-  (*     match e with *)
-  (*     | Arc.InsSem.RegERead rslc => *)
+  Definition handle_memE {E} `{threadE -< E} `{nondetFinE -< E}
+    : Arc.InsSem.memE ~> itree E :=
+    fun _ e =>
+      match e with
+      | Arc.InsSem.MemERead loc => (* FIXME: InsSem should use slc instead of loc *)
+        handle_mem_read {| Arc.location := loc;
+                           Arc.size := 1 |}
+      | Arc.InsSem.MemEWrite loc val => ITree.spin (* FIXME: *)
+      end.
 
-  (*       Ret (read_reg_slc rslc iid s) *)
-  (*     | Arc.InsSem.RegEWrite rslc rval => Ret (write_reg_slc rslc rval iid s, tt) *)
-  (*     end. *)
+  Definition lift_ins_sem {E} `{threadE -< E} `{nondetFinE -< E}
+    : itree Arc.InsSem.E ~> itree E :=
+    fun _ it =>
+      let h := case_ handle_regE handle_memE in
+      interp h it.
 
-  Definition new_instruction
-    : ktree SE (instruction_id_t * Arc.InsSem.pc_t) Types.result :=
+  Definition new_instruction {E}
+             `{wrapE threadE instruction_id_t -< E} `{nondetFinE -< E}
+    : ktree (schedulerE (instruction_id_t * Arc.InsSem.pc_t) +' E)
+            (instruction_id_t * Arc.InsSem.pc_t)
+            (Types.result unit unit) :=
     fun '(id, loc) =>
-      mem_val <- trigger (Wrap (ThEInsFetch loc) id)
-      ;; ast <- trigger (Wrap (ThEInsDecode mem_val) id)
-      ;; next_ins <- trigger (Wrap (ThEInsNextLocs loc ast) id)
-      ;; ITree.iter (fun next_ins =>
-                       match next_ins with
-                       | [] => ret (inr tt)
-                       | (id, loc)::next_ins => trigger (Spawn (id, loc))
-                                              ;; ret (inl next_ins)
-                       end) next_ins
-      ;; resum_it _ (translate (fun _ e => Wrap e id) (Arc.InsSem.denote ast)
-                    ;; ret Accept).
+      let it : itree (threadE +' nondetFinE +' schedulerE (instruction_id_t * Arc.InsSem.pc_t))
+                     (Types.result unit unit) :=
+          mem_val <- trigger (ThEInsFetch loc)
+          ;; ast <- trigger (ThEInsDecode mem_val)
+          ;; next_ins <- trigger (ThEInsNextLocs loc ast)
+          ;; ITree.iter (fun next_ins =>
+                           match next_ins with
+                           | [] => ret (inr tt)
+                           | (nid, nloc)::next_ins => trigger (Spawn (nid, nloc))
+                                                    ;; ret (inl next_ins)
+                           end) next_ins
+          ;; 'tt <- resum_it _ (lift_ins_sem _ (Arc.InsSem.denote ast))
+          ;; 'tt <- trigger ThEInsFinish
+          ;; ret (Accept tt) in
+      (* Finnaly, wrap the threadE events with the iid *)
+      resum_it _ (wrap_event_in_it threadE id _ it).
 
-  Definition denote
-    : ktree SE (instruction_id_t * Arc.InsSem.pc_t) Types.result :=
-    fun '(id, loc) => nondet_scheduler new_instruction [new_instruction (id, loc)].
+  Definition denote {E}
+             `{wrapE threadE instruction_id_t -< E} `{nondetFinE -< E}
+    : ktree E (instruction_id_t * Arc.InsSem.pc_t) (Types.result unit unit) :=
+    fun '(id, loc) =>
+      resum_it _ (scheduler new_instruction
+                            (fun r1 r2 => match r1, r2 with
+                                       | Accept tt, Accept tt => Accept tt
+                                       | _, _ => Reject tt
+                                       end)
+                            (Accept tt)
+                            [new_instruction (id, loc)]).
 End Denote.
 
 (*******************************************************************************)
@@ -131,8 +178,8 @@ Module State(Arc : ArcSig).
   | IESMemRead : instruction_exec_state
   | IESMemWrite : instruction_exec_state.
 
-  Record fetched_instruction_state :=
-    mk_fetched_instruction_state {
+  Record decoded_instruction_state :=
+    mk_decoded_instruction_state {
         ins_id : instruction_id_t;
         ins_loc : Arc.mem_loc; (*: record fetched address :*)
         (* statically analysed data about the instruction*)
@@ -159,12 +206,12 @@ Module State(Arc : ArcSig).
 
         ins_exec_state: instruction_exec_state }.
 
-  Instance eta_fetched_instruction_state : Settable _ :=
-    settable! mk_fetched_instruction_state <ins_id; ins_loc; ins_kind; ins_regs_in; ins_regs_feeding_address; ins_regs_out; ins_mem_reads; ins_mem_writes; ins_finished; ins_exec_state>.
+  Instance eta_decoded_instruction_state : Settable _ :=
+    settable! mk_decoded_instruction_state <ins_id; ins_loc; ins_kind; ins_regs_in; ins_regs_feeding_address; ins_regs_out; ins_mem_reads; ins_mem_writes; ins_finished; ins_exec_state>.
 
-  Definition initial_fetched_instruction_state (loc : Arc.mem_loc)
+  Definition initial_decoded_instruction_state (loc : Arc.mem_loc)
              (ast : Arc.InsSem.ast)
-    : fetched_instruction_state :=
+    : decoded_instruction_state :=
     let '(regs_in, regs_feeding_address, regs_out) := Arc.InsSem.regs_from_ast ast in
     (* instruction_state: *)
     {| ins_id := 0; (* FIXME: get fresh id *)
@@ -180,7 +227,8 @@ Module State(Arc : ArcSig).
 
   Variant instruction_state :=
   | ISUnfetched : Arc.mem_loc -> instruction_state
-  | ISFetched : fetched_instruction_state -> instruction_state.
+  | ISFetched : Arc.mem_loc -> Arc.InsSem.machine_code -> instruction_state
+  | ISDecoded : decoded_instruction_state -> instruction_state.
 
   Record state :=
     mk_state {
@@ -215,6 +263,40 @@ Module State(Arc : ArcSig).
       | Arc.InsSem.RegEWrite rslc rval => Ret (write_reg_slc rslc rval iid s, tt)
       end.
 
+  Definition handle_threadE {E}
+    : wrapE ThrDenote.threadE Thread.instruction_id_t ~>
+            stateT state (itree E) :=
+    fun _ e s =>
+      let '(Wrap e iid) := e in
+      match e with
+      | ThEInsFetch _ => ITree.spin
+      | ThEInsReadFromSto _ => ITree.spin
+
+      | ThEInsDecode code =>
+        match Arc.InsSem.decode code with
+        | Some ast =>
+          (* FIXME: update [s] *)
+          Ret (s, ast)
+        | None => throw InsDecodeFail
+        end
+
+      | ThEInsNextLocs loc ast =>
+        let next_pcs := Arc.InsSem.next_pc loc ast in
+        let iids := List.seq s.(next_iid) (List.length next_pcs) in
+        let s := s <| next_iid := s.(next_iid) + (List.length next_pcs) |> in
+        Ret (s, list.compose iids next_pcs)
+
+      | ThEInsDecode : Arc.InsSem.machine_code -> threadE Arc.InsSem.ast
+      | ThEInsNextLocs : Arc.InsSem.pc_t -> Arc.InsSem.ast ->
+                         threadE (list (instruction_id_t * Arc.InsSem.pc_t))
+      | ThEInsFinish : threadE unit
+      (* Load instruction *)
+      | ThEInsInitReads : Arc.mem_slc -> threadE (list mem_read_id_t)
+      | ThEInsWriteForward : mem_read_id_t -> threadE bool
+      | ThEGetValueOfReads : threadE Arc.mem_slc_val.
+
+      end.
+
   (* Definition handle_thread {E} : Arc.InsSem.E ~> stateT thread_state (itree E) :=. *)
 
   (* Definition handle_thread {E} : threadE ~> stateT thread_state (itree E) := *)
@@ -229,5 +311,6 @@ Module State(Arc : ArcSig).
   (* *) *)
   (* Definition interp_map {E d} : itree (mapE d +' E) ~> stateT map (itree E) := *)
   (*   interp_state (case_ handle_map pure_state). *)
+
 
 End State.
