src/Storage.v
@@ -1,5 +1,5 @@
 From Coq Require Import
-     Arith.PeanoNat
+     Arith
      NArith.NArith
      Lists.List
      Lists.ListSet
@@ -32,9 +32,36 @@ Local Open Scope monad_scope.
 (* Local Open Scope monad_scope. *)
 
 Module State (Arc : ArcSig).
+  (* `mem` is a map from byte locations to byte values *)
   Record state := mk_state { mem : Arc.mem_loc -> option Arc.mem_slc_val }.
   Instance eta_state : Settable _ := settable! mk_state <mem>.
 
   Definition initial_state (mem : Arc.mem_loc -> option Arc.mem_slc_val) : state :=
     {| mem := mem |}.
+
+  (* Head of `svs` is most significant *)
+  Definition combine_values (svs : list (nat * option Arc.mem_slc_val))
+    : option (nat * Arc.mem_slc_val) :=
+    List.fold_left
+        (fun acc sv =>
+           match acc, sv with
+           | Some (acc_size, acc_val), (size, Some val) =>
+             Some (acc_size + size, acc_val * (2 ^ (8 * size)) + val)
+           | _, _ => None
+           end)
+        svs
+        (Some (0, 0)).
+
+  Definition get_slc (slc : Arc.mem_slc) (s : state) : option (nat * Arc.mem_slc_val) :=
+    let bytes := List.map (fun o => (1, s.(mem) (slc.(Arc.location) + o)))
+                          (List.seq 0 slc.(Arc.size)) in
+    combine_values
+      (* TODO: the `rev` is because we assume little-endianness *)
+      (List.rev bytes).
+
+  Definition read_instruction (loc : Arc.mem_loc) (s : state) : option (nat * Arc.mem_slc_val) :=
+    (* TODO: we assume all instructions are 4 bytes *)
+    let ins_size := 4 in
+    get_slc ({| Arc.location := loc; Arc.size := ins_size |}) s.
+
 End State.
