src/System.v
@@ -51,21 +51,34 @@ Module System (Arc : ArcSig).
   Module ThrDenote := Thread.Denote Arc.
   Definition thread_id_t := Utils.id_t.
 
+  Definition thread_it {E}
+             `{wrapE ThrDenote.threadE (Thread.instruction_id_t * thread_id_t) -< E}
+             `{nondetFinE -< E}
+             '((loc, tid) : nat * thread_id_t)
+    : itree E (Types.result unit unit) :=
+    (* TODO: convert loc from nat to Arc.InsSem.pc_t *)
+    let it := ThrDenote.denote (0, loc) in
+    let it := map_wrap_event_in_it ThrDenote.threadE (fun iid => (iid, tid)) _ it in
+    resum_it _ it.
+
   Definition denote {E}
-             `{wrapE ThrDenote.SE thread_id_t -< E}
+             `{wrapE ThrDenote.threadE (Thread.instruction_id_t * thread_id_t) -< E}
+             `{nondetFinE -< E}
              (entry_locs : list nat)
-    : itree (nondet_schedulerE unit +' E) unit :=
-    List.length entry_locs
-    $> List.seq 0
-    $> List.combine entry_locs
-    $> List.map (fun '(eloc, tid) => wrap_it tid _ (ThrDenote.denote (0, eloc)))
-    $> nondet_scheduler (fun tt => ITree.spin).
-       (* The spin is unreachable.
-          TODO: do we want to support spawning of new threads?
-          Probably not. *)
-
-
-
+    : itree E unit :=
+    let it :=
+        List.length entry_locs
+        $> List.seq 0
+        $> List.combine entry_locs
+        $> List.map thread_it
+        $> scheduler
+             (fun 'tt => ITree.spin) (* spawn *)
+                    (* The spin is unreachable.
+                       TODO: do we want to support spawning of new threads?
+                       Probably not. *)
+             (fun 'tt _ => tt) (* fold_results *)
+             tt in (* acc_result *)
+    resum_it _ it.
 
   Module ThrState := Thread.State Arc.
   Module StoState := Storage.State Arc.
@@ -84,67 +97,65 @@ Module System (Arc : ArcSig).
     {| storage := StoState.initial_state mem;
        threads := List.map ThrState.initial_state entry_locs |}.
 
-  Definition handle_thr_regE {E}
-    : wrapE (wrapE Arc.InsSem.regE Thread.instruction_id_t) thread_id_t ~> stateT state (itree E) :=
-    fun _ e s =>
-      let '(Wrap e tid) := e in
-      match List.nth_error s.(threads) tid with
-      | Some thr_state =>
-        '(thr_state, a) <- ThrState.handle_regE _ e thr_state
-        ;; let ts := list_replace_nth tid thr_state s.(threads) in
-           Ret (s <| threads := ts |>, a)
-      | None => ITree.spin (* Unreachable *)
-      end.
 
-  Definition handle_thr_memE {E}
-    : wrapE (wrapE Arc.InsSem.memE Thread.instruction_id_t) thread_id_t ~> stateT state (itree E) :=
-    fun _ e s =>
-      let '(Wrap e tid) := e in
-      match List.nth_error s.(threads) tid with
-      | Some thr_state =>
-        '(thr_state, a) <- ThrState.handle_memE _ e thr_state
-        ;; let ts := list_replace_nth tid thr_state s.(threads) in
-           Ret (s <| threads := ts |>, a)
-      | None => ITree.spin (* Unreachable *)
-      end.
+  (* Definition handle_thr_memE {E} *)
+  (*   : wrapE (wrapE Arc.InsSem.memE Thread.instruction_id_t) thread_id_t ~> stateT state (itree E) := *)
+  (*   fun _ e s => *)
+  (*     let '(Wrap e tid) := e in *)
+  (*     match List.nth_error s.(threads) tid with *)
+  (*     | Some thr_state => *)
+  (*       '(thr_state, a) <- ThrState.handle_memE _ e thr_state *)
+  (*       ;; let ts := list_replace_nth tid thr_state s.(threads) in *)
+  (*          Ret (s <| threads := ts |>, a) *)
+  (*     | None => ITree.spin (* Unreachable *) *)
+  (*     end. *)
 
   Definition handle_threadE {E}
-    : wrapE (wrapE ThrDenote.threadE Thread.instruction_id_t) thread_id_t ~> stateT state (itree E) :=
+             `{exceptE disabled -< E}
+             `{exceptE system_deadlock -< E}
+    : wrapE ThrDenote.threadE (Thread.instruction_id_t * thread_id_t) ~>
+            stateT state (itree E) :=
     fun _ e s =>
-      let '(Wrap e tid) := e in
+      let '(Wrap e (iid, tid)) := e in
       match List.nth_error s.(threads) tid with
       | Some thr_state =>
-        let '(Wrap e iid) := e in
         match e with
-        | ThEFetch loc => Ret(s, 0%N) (* FIXME: *)
-        | ThEDecode code => Ret(s, Arc.InsSem.decode code)
-        | ThENextLocs loc ast =>
-          let next_pcs := Arc.InsSem.next_pc loc ast in
-          let iids := List.seq thr_state.(next_iid) (List.length next_pcs) in
-          let thr_state := thr_state <| next_iid := thr_state.(next_iid) + (List.length next_pcs) |> in
-          let ts := list_replace_nth tid thr_state s.(threads) in
-          Rest(s <| thread := ts |>, list.compose iids next_pcs)
+        | ThEInsFetch loc =>
+          match StoState.read_instruction loc s.(storage) with
+          | Some (size, code) =>
+            (* TODO: pass `size` to the thread so it knows how to increment the PC. *)
+            '(thr_state, answer) <- ThrState.handle_ThEInsFetch size code iid thr_state
+            ;; let ts := list_replace_nth tid thr_state s.(threads) in
+               Ret (s <| threads := ts |>, answer)
+
+            Ret (s, code)
+          | None => throw InsNotInStorage
+          end
+
+        | ThEInsReadFromSto rid =>
+          match ThrState.handle_ThEInsReadFromSto rid iid thr_state with
+          | Some (thr_state, read_request) =>
+            match StoState.read_data read_request s.(storage) with
+            | Some (size, val) =>
+              let ts := list_replace_nth tid (thr_state val) s.(threads) in
+              Ret (s <| threads := ts |>, true)
+            | None => throw ReadFromUnmappedMem
+            end
+          | None => throw Disabled
+          end
+
+        | _ =>
+          '(thr_state, answer) <- ThrState.handle_threadE e iid thr_state
+          ;; let ts := list_replace_nth tid thr_state s.(threads) in
+             Ret (s <| threads := ts |>, answer)
         end
       | None => ITree.spin (* Unreachable *)
       end.
 
+  Definition interp_system {E}
+    : itree (wrapE ThrDenote.threadE (Thread.instruction_id_t * thread_id_t) +' E) ~>
+            stateT state (itree E) :=
+    interp_state (case_ handle_threadE pure_state).
 
-
-
-
-
-
-
-      Definition interp_system {E}
-                 (it : itree (systemE +' E) unit)
-        : system_state -> itree E (system_state * unit) :=
-        let h := bimap h_reg (bimap h_memory (id_ _)) in
-        let it := interp h it in
-        fun s => interp_map (interp_map t' regs) mem.
-
-
-      (** We can then define an evaluator for closed assembly programs by interpreting
-    both store and heap events into two instances of [mapE], and running them
-    both in the empty initial environments.  *)
-      Definition run_system (mem : nat -> option nat) (entry_locs : list nat) :=
-        interp_system (denote entry_locs) (initial_state mem entry_locs).
+  Definition run_system (mem : nat -> option nat) (entry_locs : list nat) :=
+    interp_system (denote entry_locs) (initial_state mem entry_locs).
